Clean up, and polymorphism example

theories/logrel/examples/mapper.v
@@ -1,32 +1,22 @@
 From actris.channel Require Import proofmode proto channel.
-From actris.logrel Require Import subtyping_rules term_typing_judgment term_typing_rules environments operators.
+From actris.logrel Require Import subtyping_rules term_typing_judgment term_typing_rules environments operators subtyping_rules.
 From iris.proofmode Require Import tactics.
 
 Section with_Σ.
   Context `{heapG Σ, chanG Σ}.
 
+  (** Client typing *)
   Definition mapper_client_type_aux (rec : lsty Σ) : lsty Σ :=
     <!!> TY (lty_int ⊸ lty_bool); <!!> TY lty_int; <??> TY lty_bool; rec.
   Definition mapper_client_type : lsty Σ :=
     mapper_client_type_aux END.
-
   Instance mapper_client_type_contractive : Contractive mapper_client_type_aux.
   Proof. solve_proto_contractive. Qed.
-
   Definition mapper_client_rec_type : lsty Σ :=
     lty_rec mapper_client_type_aux.
 
-  Definition mapper_service_type : lsty Σ :=
-    <??> TY (lty_int ⊸ lty_bool); <??> TY lty_int; <!!> TY lty_bool; END.
-
   Definition mapper_client : expr := λ: "c",
-    send "c" (λ: "x", #9000 < "x");;
-    send "c" #42;; recv "c".
-
-  Definition mapper_service : expr := λ: "c",
-    let: "f" := recv "c" in
-    let: "v" := recv "c" in
-    send "c" ("f" "v");; "c".
+    send "c" (λ: "x", #9000 < "x");; send "c" #42;; recv "c".
 
   Lemma mapper_client_typed Γ :
     ⊢ Γ ⊨ mapper_client : (lty_chan (mapper_client_type) ⊸ lty_bool)%lty ⫤ Γ.
@@ -50,36 +40,7 @@ Section with_Σ.
     rewrite insert_insert /=. iApply ltyped_recv. apply lookup_insert.
   Qed.
 
-  Lemma mapper_service_typed Γ :
-    ⊢ Γ ⊨ mapper_service : (lty_chan (mapper_service_type) ⊸ (lty_chan END))%lty ⫤ Γ.
-  Proof.
-    iApply (ltyped_frame _ _ _ _ Γ).
-    { iApply env_split_id_l. }
-    2: { iApply env_split_id_l. }
-    iApply ltyped_lam.
-    iApply ltyped_let.
-    { iApply ltyped_recv. by rewrite lookup_insert. }
-    rewrite insert_insert /=.
-    iApply ltyped_let.
-    { iApply ltyped_recv. by rewrite insert_commute // lookup_insert. }
-    rewrite (insert_commute _ "c" "f") // insert_insert.
-    iApply ltyped_let=> /=; last first.
-    { iApply ltyped_var. apply lookup_insert. }
-    iApply ltyped_send. apply lookup_insert.
-    rewrite (insert_commute _ "f" "c") // (insert_commute _ "v" "c") //.
-    iApply (ltyped_frame _ _ _ _ {["c":=_]}).
-    { iApply env_split_right=> //. iApply env_split_id_r. }
-    { iApply ltyped_app.
-      - iApply ltyped_var. apply lookup_insert.
-      - rewrite insert_commute //.
-        iApply (ltyped_frame _ _ _ _ {["f":=_]}).
-        { iApply env_split_right=> //. iApply env_split_id_r. }
-        { iApply ltyped_var. apply lookup_insert. }
-        { iApply env_split_right=> //; last by iApply env_split_id_r. eauto. }
-    }
-    { iApply env_split_right=> //; last by iApply env_split_id_r. eauto. }
-  Qed.
-
+  (** Recursion and Swapping *)
   Lemma lty_le_rec_unfold_l {k} (C : lty Σ k → lty Σ k) `{!Contractive C} :
     ⊢ lty_rec C <: C (lty_rec C).
   Proof. iApply lty_le_l. iApply lty_le_rec_unfold. iApply lty_le_refl. Qed.
@@ -112,7 +73,7 @@ Section with_Σ.
         { iModIntro. iApply lty_le_rec_unfold_l. }
         iApply lty_le_trans. iApply lty_le_swap_recv_send. iModIntro.
         iApply lty_le_trans. iApply lty_le_swap_recv_send. iModIntro.
-        iModIntro. iModIntro. iApply lty_le_refl.
+        eauto.
       - iApply lty_le_refl. }
     iApply ltyped_lam.
     iApply ltyped_let.
@@ -125,8 +86,7 @@ Section with_Σ.
       { iApply env_split_id_l. } }
     rewrite insert_insert /=.
     iApply ltyped_let.
-    { iApply ltyped_send. apply lookup_insert.
-      iApply ltyped_int. }
+    { iApply ltyped_send. apply lookup_insert. iApply ltyped_int. }
     rewrite insert_insert /=.
     iApply ltyped_let.
     { iApply ltyped_send. apply lookup_insert.
@@ -155,5 +115,135 @@ Section with_Σ.
       iApply ltyped_var. apply lookup_insert.
       iApply env_split_right=> //; last by iApply env_split_id_r=> //=. eauto.
   Qed.
+
+  Definition mapper_client_type_poly_aux (rec : lsty Σ) : lsty Σ :=
+    <!! X Y> TY (X ⊸ Y); <!!> TY X; <??> TY Y; rec.
+
+  Instance mapper_client_type_poly_contractive :
+    Contractive mapper_client_type_poly_aux.
+  Proof. solve_proto_contractive. Qed.
+
+  Definition mapper_client_rec_type_poly : lsty Σ :=
+    lty_rec mapper_client_type_poly_aux.
+
+  Definition mapper_client_type_poly_swap (rec : lsty Σ) : lsty Σ :=
+    <!!> TY (lty_int ⊸ lty_bool); <!!> TY lty_int;
+    <!!> TY (lty_bool ⊸ lty_int); <!!> TY lty_bool;
+    <??> TY lty_bool; <??> TY lty_int; rec.
+
+  Definition mapper_client_rec_poly : expr := λ: "c",
+    send "c" (λ: "x", #9000 < "x");; send "c" #42;;
+    send "c" (λ: "x", if: #true then #1 else #0);; send "c" #true;;
+    let: "x" := recv "c" in
+    let: "y" := recv "c" in
+    ("x","y").
+
+  Lemma mapper_client_rec_poly_typed Γ :
+    ⊢ Γ ⊨ mapper_client_rec_poly :
+      (lty_chan (mapper_client_rec_type_poly) ⊸ (lty_bool * lty_int))%lty ⫤ Γ.
+  Proof.
+    iApply (ltyped_frame _ _ _ _ Γ).
+    { iApply env_split_id_l. }
+    2: { iApply env_split_id_l. }
+    iApply (ltyped_subsumption _ _ _
+      ((lty_chan (mapper_client_type_poly_swap mapper_client_rec_type_poly)) ⊸ _)).
+    { iApply lty_le_arr.
+      - iNext. iApply lty_le_chan. iNext.
+        iApply lty_le_trans. iApply lty_le_rec_unfold_l.
+        rewrite /mapper_client_type_poly_aux.
+        rewrite /mapper_client_type_poly_swap.
+        iExists lty_int, lty_bool.
+        iModIntro. iModIntro.
+        iApply lty_le_trans.
+        { iModIntro. iApply lty_le_rec_unfold_l. }
+        iApply lty_le_trans; last first.
+        { iModIntro. iApply lty_le_swap_recv_send. }
+        iApply lty_le_trans; last first.
+        { iApply lty_le_swap_recv_send. }
+        iModIntro.
+        iExists lty_bool, lty_int.
+        iApply lty_le_refl.
+      - iApply lty_le_refl. }
+    iApply ltyped_lam.
+    iApply ltyped_let.
+    { iApply ltyped_send. apply lookup_insert.
+      iApply (ltyped_frame _ _ _ _ {["c":=_]}).
+      { iApply env_split_id_l. }
+      { iApply ltyped_lam. iApply ltyped_bin_op.
+        - iApply ltyped_var. apply lookup_insert.
+        - iApply ltyped_int. }
+      { iApply env_split_id_l. } }
+    rewrite insert_insert /=.
+    iApply ltyped_let.
+    { iApply ltyped_send. apply lookup_insert.
+      iApply ltyped_int. }
+    rewrite insert_insert /=.
+    iApply ltyped_let.
+    { iApply ltyped_send. apply lookup_insert.
+      iApply (ltyped_frame _ _ _ _ (<["c":=_]>∅)).
+      { iApply env_split_id_l. }
+      { iApply ltyped_lam. iApply ltyped_if.
+        - iApply ltyped_bool.
+        - iApply ltyped_int.
+        - iApply ltyped_int. }
+      { iApply env_split_id_l. } }
+    rewrite insert_insert /=.
+    iApply ltyped_let.
+    { iApply ltyped_send. apply lookup_insert. iApply ltyped_bool. }
+    rewrite insert_insert /=.
+    iApply ltyped_let.
+    { iApply ltyped_recv. apply lookup_insert. }
+    rewrite insert_insert /=.
+    iApply ltyped_let.
+    { iApply ltyped_recv=> //. }
+    iApply ltyped_pair.
+    - iApply ltyped_var. apply lookup_insert.
+    - rewrite (insert_commute _ "c" "x") //= (insert_commute _ "y" "x") //=.
+      rewrite insert_insert.
+      iApply (ltyped_frame _ _ _ _ {["x":=_]}).
+      { iApply env_split_right=> //=. iApply env_split_id_r. }
+      iApply ltyped_var. apply lookup_insert.
+      iApply env_split_right=> //; last by iApply env_split_id_r=> //=. eauto.
+  Qed.
+
+  (** Service typing *)
+  Definition mapper_service_type : lsty Σ :=
+    <??> TY (lty_int ⊸ lty_bool); <??> TY lty_int; <!!> TY lty_bool; END.
+
+  Definition mapper_service : expr := λ: "c",
+    let: "f" := recv "c" in
+    let: "v" := recv "c" in
+    send "c" ("f" "v");; "c".
+
+  Lemma mapper_service_typed Γ :
+    ⊢ Γ ⊨ mapper_service : (lty_chan (mapper_service_type) ⊸ (lty_chan END))%lty ⫤ Γ.
+  Proof.
+    iApply (ltyped_frame _ _ _ _ Γ).
+    { iApply env_split_id_l. }
+    2: { iApply env_split_id_l. }
+    iApply ltyped_lam.
+    iApply ltyped_let.
+    { iApply ltyped_recv. by rewrite lookup_insert. }
+    rewrite insert_insert /=.
+    iApply ltyped_let.
+    { iApply ltyped_recv. by rewrite insert_commute // lookup_insert. }
+    rewrite (insert_commute _ "c" "f") // insert_insert.
+    iApply ltyped_let=> /=; last first.
+    { iApply ltyped_var. apply lookup_insert. }
+    iApply ltyped_send. apply lookup_insert.
+    rewrite (insert_commute _ "f" "c") // (insert_commute _ "v" "c") //.
+    iApply (ltyped_frame _ _ _ _ {["c":=_]}).
+    { iApply env_split_right=> //. iApply env_split_id_r. }
+    { iApply ltyped_app.
+      - iApply ltyped_var. apply lookup_insert.
+      - rewrite insert_commute //.
+        iApply (ltyped_frame _ _ _ _ {["f":=_]}).
+        { iApply env_split_right=> //. iApply env_split_id_r. }
+        { iApply ltyped_var. apply lookup_insert. }
+        { iApply env_split_right=> //; last by iApply env_split_id_r. eauto. }
+    }
+    { iApply env_split_right=> //; last by iApply env_split_id_r. eauto. }
+  Qed.
+
 
 End with_Σ.
